\documentclass[Aluffi.tex]{subfiles}

\begin{document}

\section{II: Rings and Modules}

\subsection{Section 5}

\begin{problem}
Let $R$  be a commutative ring, viewed as a $R$-module over itself and let $M$ be an $R$-module.
Prove that $Hom_{R_{Mod}}(R.M) \cong M$ as an isomorphism of $R$-modules.
\end{problem}

\begin{proof}
Consider the map $\phi: Hom_{R_{Mod}}(R,M) \rightarrow M$ that takes $\psi_m$ which is a $R$-module homomorphism from $R \rightarrow M$ such that $\psi_m(1_R)= m$ where $1_R$ is the multiplicative unit of $R$
to $m$ itself. We see that such a map is indeed a homomorphism as $\phi(\psi_m   \circ \psi_n)= \phi(\psi_{mn}) = mn = \phi(\psi_m)\phi(\psi_n)$. Injectivity follows from our definition as we map the $R$'s unit to $m$. This induces an unique $R$-module homomorphism. Surjectivity follows as well as any such $\psi
_{m} \in Hom_{R_{Mod}}(R,M)$. Thus, as $\phi$ is a bijective homomorphism, it follows that it is a $R$-module isomorphism.
\end{proof}

\begin{problem}
Let $R$ be a commutative ring and let $M$ be an $R$-module. Prove that the operation of composition on the $R$-module $End_{R_{Mod}}(M)$ makes the latter into an $R$-algebra in a natural way.
\end{problem}

\begin{proof}
Given the $R$-module $End_{R_{Mod}}(M)$, we shall prove that the multiplicative operation of composition (which turns $End_{R_{Mod}}(M)$ into a ring), turns it into an $R$-algebra. Given any $\phi \in End_{R_{Mod}}(M)$. For any given $\phi_1,\phi_2 \in End_{R_{Mod}}(M), m \in M$ $a \in R$, then  $(r\phi_1)(m) \circ \phi_)(m)  = (r\phi_1)(a\phi_2(m)) = r\phi_1a(\phi_2(m)) = ra(\phi_1(m) \circ \phi_2(m))$ (???). (consider acrion of $r$ on composition to get equality)
\end{proof}

\begin{problem}
Let $R$ be an integral domain and let $I$ be a nonzero principal domain of $R$. Prove that $I$ is isomorphic to $R$ as an $R$-module.
\end{problem}

\begin{proof}
Let $I = (i)$ be our principal ideal in $R$. Consider the map $\phi: R \rightarrow I$ as $r \mapsto ri$. This map can be easily shown to be an abelian group homomorphism. Also for $s \in R$, $\phi(sr) = sri = s(ri) = s \phi(r)$. Thus, $\phi$ is also a $R$-module homomorphism. Injectivity of our map follows from the assumption that $R$ is an integral domain and $i \neq 0$. Surjectivity follows as $\{ri \vert r \in R\} = I$. Thus, $\phi$ is a $R$-module isomorphism. 
\end{proof}

\begin{problem}
Let $R$ be a commutative ring. $M$ be a $R$-module, and let $a \in R$ be a nilpotent element, determining a submodule $aM$ of $M$. Prove that $M = 0$ iff $aM = M$. (This is a special case of Nakayama's Lemma)
\end{problem}

\begin{proof}
If $M = 0$, then it trivially implies that $aM =M$. Conversely, let $M \neq 0$ and $aM = M$, then there exists  nonzero elements $m,m_1 \in M$ such that $m = am_1$. By the same argument, there exists nonzero $m_2$
such that $m_1 = am_2$. Continue this procedure for $n$ steps where $a^n = 0$. Then we have that $m = a^nm_n = 0$, contradicting our assumption above. Hence, $M = 0$ exactly.
\end{proof}

\begin{problem}
Let $R$ be a commutatative ring and let $I$ be an ideal of $R$. Noting that $I^j \cdot I^k \subseteq I^{jk}$,
define a ring structure on the direct sum 
$$\text{Rees}_R(I) = \bigoplus_{j \geq 0} I^j = R \oplus I \oplus I^2 \oplus ...$$
By embedding $R$ into the first term, we create an $R$-algebra, called the Rees Algebra of $I$. Prove that if $a \in R$ is a nonzero divisor, then $Rees_{R}((a)) \cong R[x]$ as an $R$-algebra isomorphism. 
\end{problem}

\begin{proof}
Consider the map $F: \text{Rees}_R((a)) \rightarrow R[x]$ that takes $s_i = (0,0,0,...,1_Ra^i,...) \mapsto x^i$ for $i \geq 0$.  Consider the definition of the Rees and algebra and note that 
$ I = \{ri \vert i \in I\}$, $I^2 = \{\sum_{r,t \in R,finite} ra \cdot ta \}$ and hence forth. This exactly concides with multiplication operation on elements in the ring $R[X]$. Hence, the map is a surjective ring homomorphism. Injectivity follows from the assumption that $a$ is a non-zero divisor in $R$. The map preserves the $R$-module structure and thus is an $R$-algebra isomorphism.  
\end{proof}





\end{document}